Turn `normalisation` into a typeclass
We use two typeclasses: one for specifying that we can achieve
normalisation within a particular environment, while the other posits
normalisation for all well-formed environments.  This is useful because
while the latter is expected to be unprovable, it may be possible to
prove that specific concrete environments are normalising, which may
allow us to prove particular programs well-typed more easily without
axioms.

erasure/theories/ETransform.v
@@ -20,14 +20,14 @@ Definition build_wf_env_from_env {cf : checker_flags} (Σ : global_env_map) (wf�
      wf_env_map_repr := Σ.(trans_env_repr);
  |}.
 
-Program Definition erase_pcuic_program {guard : abstract_guard_impl} (p : pcuic_program)
+Program Definition erase_pcuic_program {guard : abstract_guard_impl} {normalisation : PCUICSN.Normalisation} (p : pcuic_program)
   (wfΣ : ∥ PCUICTyping.wf_ext (H := config.extraction_checker_flags) p.1 ∥)
   (wt : ∥ ∑ T, PCUICTyping.typing (H := config.extraction_checker_flags) p.1 [] p.2 T ∥) : eprogram_env :=
   let wfe := build_wf_env_from_env p.1.1 (map_squash (PCUICTyping.wf_ext_wf _) wfΣ) in
   let wfext := @abstract_make_wf_env_ext _ optimized_abstract_env_impl wfe p.1.2 _ in
-  let t := ErasureFunction.erase (nor:=PCUICSN.extraction_normalizing) optimized_abstract_env_impl wfext nil p.2
+  let t := ErasureFunction.erase (nor:=PCUICSN.extraction_normalizing) (normalisation_in:=let _ := @PCUICSN.normalisation in _) optimized_abstract_env_impl wfext nil p.2
     (fun Σ wfΣ => let '(sq (T; ty)) := wt in PCUICTyping.iswelltyped ty) in
-  let Σ' := ErasureFunction.erase_global_fast optimized_abstract_env_impl
+  let Σ' := ErasureFunction.erase_global_fast (nor:=PCUICSN.extraction_normalizing) (normalisation:=normalisation) optimized_abstract_env_impl
     (EAstUtils.term_global_deps t) wfe (p.1.(PCUICAst.PCUICEnvironment.declarations)) _ in
     (EEnvMap.GlobalContextMap.make Σ' _, t).
 
@@ -40,11 +40,11 @@ Obligation Tactic := idtac.
 
 Import Extract.
 
-Definition erase_program {guard : abstract_guard_impl} (p : pcuic_program)
+Definition erase_program {guard : abstract_guard_impl} {normalisation : PCUICSN.Normalisation} (p : pcuic_program)
   (wtp : ∥ wt_pcuic_program (cf:=config.extraction_checker_flags) p ∥) : eprogram_env :=
   erase_pcuic_program (guard := guard) p (map_squash fst wtp) (map_squash snd wtp).
 
-Lemma expanded_erase_program {guard : abstract_guard_impl}
+Lemma expanded_erase_program {guard : abstract_guard_impl} {normalisation : PCUICSN.Normalisation}
   (cf := config.extraction_checker_flags) p (wtp : ∥ wt_pcuic_program p ∥) :
   PCUICEtaExpand.expanded_pcuic_program p ->
   EEtaExpandedFix.expanded_eprogram_env (erase_program (guard:=guard) p wtp).
@@ -67,7 +67,7 @@ Proof.
   - eapply EEtaExpanded.isEtaExpFix_isEtaExp. now eapply EEtaExpandedFix.expanded_isEtaExp.
 Qed.
 
-Program Definition erase_transform {guard : abstract_guard_impl}  : Transform.t pcuic_program eprogram_env PCUICAst.term EAst.term
+Program Definition erase_transform {guard : abstract_guard_impl} {normalisation : PCUICSN.Normalisation} : Transform.t pcuic_program eprogram_env PCUICAst.term EAst.term
   eval_pcuic_program (eval_eprogram_env EWcbvEval.default_wcbv_flags) :=
  {| name := "erasure";
     pre p :=
@@ -77,7 +77,7 @@ Program Definition erase_transform {guard : abstract_guard_impl}  : Transform.t 
     obseq g g' v v' := let Σ := g.1 in Σ ;;; [] |- v ⇝ℇ v' |}.
 Next Obligation.
   cbn -[erase_program].
-  intros ? p [wtp etap].
+  intros ? ? p [wtp etap].
   destruct erase_program eqn:e.
   split; cbn.
   - unfold erase_program, erase_pcuic_program in e. simpl. cbn in e. injection e. intros <- <-.
@@ -89,7 +89,7 @@ Next Obligation.
 Qed.
 
 Next Obligation.
-  red. move=> guard [Σ t] v [[wf [T HT]]]. unfold eval_pcuic_program, eval_eprogram.
+  red. move=> guard normalisation [Σ t] v [[wf [T HT]]]. unfold eval_pcuic_program, eval_eprogram.
   intros [ev].
   destruct erase_program eqn:e.
   unfold erase_program, erase_pcuic_program in e. simpl in e. injection e; intros <- <-.
