safechecker/theories/PCUICSafeConversion.v
@@ -64,6 +64,8 @@ Section Conversion.
 
   Context (X : X_type.π2.π1).
 
+  Context {normalisation_in : forall Σ, wf_ext Σ -> Σ ∼_ext X -> NormalisationIn Σ}.
+
   Local Definition heΣ Σ (wfΣ : abstract_env_ext_rel X Σ) :
     ∥ wf_ext Σ ∥ :=  abstract_env_ext_wf _ wfΣ.
 
@@ -145,12 +147,12 @@ Section Conversion.
 
   Lemma wcored_wf :
     forall Γ, well_founded (wcored Γ).
-  Proof using Type.
+  Proof using normalisation_in.
     intros Γ [u hu].
     destruct (abstract_env_ext_exists X) as [[Σ wfΣ]];
-    pose proof (heΣ _ wfΣ) as heΣ.
+    pose proof (heΣ _ wfΣ) as [heΣ].
     pose proof (hu _ wfΣ) as h.
-    apply normalisation_upto in h. 2: exact heΣ.
+    apply normalisation_upto in h. 2: now apply normalisation_in.
     dependent induction h.
     constructor. intros [y hy] r.
     unfold wcored in r. cbn in r.
@@ -218,7 +220,7 @@ Section Conversion.
     forall Γ t p w q s,
       (forall Σ, abstract_env_ext_rel X Σ -> welltyped Σ Γ t) ->
       Acc (R_aux Γ) (t ; (p, (w ; (q, s)))).
-  Proof using Type.
+  Proof using normalisation_in.
     intros Γ t p w q s ht.
     destruct (abstract_env_ext_exists X) as [[Σ wfΣ]].
     rewrite R_aux_equation_1.
@@ -304,7 +306,7 @@ Section Conversion.
           -- left. unfold posR in *.
              simpl in *. assumption.
           -- right. assumption.
-    - pose proof (heΣ _ wfΣ).
+    - pose proof (heΣ _ wfΣ) as [?].
       eapply Acc_equiv; try eapply normalisation_upto; eauto.
       split; eauto; intros.
       erewrite (abstract_env_ext_irr _ _ wfΣ); eauto.
@@ -327,7 +329,7 @@ Section Conversion.
     forall Γ u,
       (forall Σ (wfΣ : abstract_env_ext_rel X Σ), welltyped Σ Γ (zipc (tm1 u) (stk1 u))) ->
       Acc (R Γ) u.
-  Proof using Type.
+  Proof using normalisation_in.
     intros Γ u h.
     eapply Acc_fun with (f := fun x => obpack x).
     apply R_aux_Acc. assumption.
@@ -2734,7 +2736,7 @@ Qed.
   Qed.
 
   Lemma welltyped_zipc_inv Σ Γ t π : wf Σ -> welltyped Σ Γ (zipc t π) -> welltyped Σ (Γ,,, stack_context π) t.
-  Proof.
+  Proof using Type.
     intros ? Ht. apply welltyped_zipc_zipp in Ht; eauto.
     apply welltyped_zipp_inv in Ht; eauto.
   Defined.
@@ -5178,7 +5180,7 @@ Qed.
   Lemma whnf_mkApps_tPrim_inv :
     forall (f : RedFlags.t) (Σ : global_env) (Γ : context) p (args : list term),
       whnf f Σ Γ (mkApps (tPrim p) args) -> args = [].
-  Proof.
+  Proof using Type.
     intros * wh.
     inversion wh; solve_discr.
     clear -X0.
